day 8

problems/8/Problem8.dfy
@@ -1,9 +1,163 @@
+include "../../parser/split.dfy"
+include "../../parser/parseInt.dfy"
+include "./QuickUnion.dfy"
+
 module Problem8 {
-    method problem8_1(input: string) returns (x: int) {
-        return 3;
+    import opened Split
+    import opened ParseInt
+    import opened Std.Collections.Seq
+    import opened QuickUnion
+
+    predicate Distinct<T(==)>(xs: seq<T>) {
+        // forall i, j :: 0 <= i  < |xs| && 0 <= j < |xs| ==> xs[i] != xs[j]
+        forall i, j :: 0 <= i <j  < |xs|  ==> xs[i] != xs[j]
     }
 
-    method problem8_2(input: string) returns (x: int) {
-        return 4;
+    method parseInput(input: string) returns (xs: seq<(nat,nat,nat)>)
+        ensures Distinct(xs)
+        ensures |xs| > 0
+    {
+        var lines := splitOnBreak(input);
+        xs := [];
+        for i := 0 to |lines| 
+            invariant Distinct(xs)
+            invariant |xs| == i
+        {
+            var coord_string := split(lines[i],",");
+            var coord := Map(Integer, coord_string);
+            expect |coord| == 3 && forall k :: 0 <= k < |coord| ==> 0 <= coord[k];
+            expect (coord[0], coord[1], coord[2]) !in xs;
+            xs := xs+[(coord[0], coord[1], coord[2])];
+        }
+        expect |xs| > 0;
+    }
+
+    function dist(a: (nat, nat, nat), b: (nat, nat, nat)): nat {
+        (a.0-b.0)*(a.0-b.0) + (a.1-b.1)*(a.1-b.1) + (a.2-b.2)*(a.2-b.2)
+    }
+
+    function min(a: nat, b: nat): nat {
+        if a < b then a else b
+    }
+
+    lemma ThereIsAMinimumTuple(s: set<(nat, nat, nat)>)
+        requires s != {}
+        ensures exists x :: x in s && forall y :: y in s ==> x.2 <= y.2
+    {
+        assert s != {};
+        var x :| x in s;
+        if s == {x} {
+        } else {
+            var s' := s - {x};
+            assert s == s' + {x};
+            ThereIsAMinimumTuple(s');
+        }
+    }
+
+    predicate gte(a: nat,b: nat) {
+        a >= b
+    }
+
+    predicate lte(a: (nat,nat,nat),b: (nat,nat,nat)) {
+        a.2 <= b.2
+    }
+
+    function AllPairs(xs: seq<(nat,nat,nat)>, i: nat): seq<(nat, nat, nat)> {
+        if xs == [] then []
+        else seq(|xs|-1, k requires 0 <= k < |xs|-1 => (i, i+k+1, dist(xs[0], xs[k+1])))+AllPairs(xs[1..], i+1)
+    }
+
+    method {:verify} problem8_1(input: string) returns (x: int) 
+        decreases *
+    {
+        x:=0;
+        var coords := parseInput(input);
+        var cmap: map<(nat, nat, nat), nat> := map i | 0 <= i < |coords| :: coords[i] := i;
+        // var pairs := set i: nat,j: nat | 0 <= i < j < |coords| :: (i,j, dist(coords[i], coords[j]));
+        var pairs := MergeSortBy(lte, AllPairs(coords, 0));
+        assert forall p :: p in pairs ==> 0 <= p.0 < p.1 < |coords|;
+        // expect pairs != {};
+        var qu := new QuickUnion(|coords|);
+        assert fresh(qu);
+        var count := 1000-1;
+        while count > 0 && pairs != [] 
+            invariant qu.Valid()
+            invariant fresh(qu)
+            invariant forall p :: p in pairs ==> 0 <= p.0 < p.1 < |coords|
+            invariant qu.n == |coords|
+            modifies qu
+            decreases *
+        {
+            var nearest := pairs[0];
+            // ThereIsAMinimumTuple(pairs);
+            // var nearest :| nearest in pairs && forall p :: p in pairs ==> nearest.2 <= p.2;
+            // print "\nnearest: ", coords[nearest.0], " ", coords[nearest.1], " ", nearest.2;
+            var areConnected := qu.connected(nearest.0, nearest.1);
+            // print "\nareConnected: ", areConnected;
+            if !areConnected {
+                qu.union(nearest.0, nearest.1);
+            }
+            count := count - 1;
+            pairs:= pairs[1..];
+
+        }
+        for i := 0 to |coords| 
+            invariant qu.Valid()
+            invariant fresh(qu)
+            invariant qu.n == |coords|
+            modifies qu
+        {
+            var root := qu.findRoot(i);
+        }
+        var counts := multiset(qu.parent[..]);
+        // print "\ncounts, ", qu.parent[..];
+        var res: seq<nat> := [];
+        while counts != multiset{} {
+            var x :| x in counts;
+            res := res + [counts[x]];
+            counts := counts[x := 0];
+        }
+        var sres := MergeSortBy(gte, res);
+        print "\n",sres,"\n";
+        return FoldLeft((a,b)=>a*b, 1, sres[..min(3, |sres|)]);
+    }
+
+    method problem8_2(input: string) returns (x: int) 
+        decreases *
+    {
+        x:=0;
+        var coords := parseInput(input);
+        var cmap: map<(nat, nat, nat), nat> := map i | 0 <= i < |coords| :: coords[i] := i;
+        // var pairs := set i: nat,j: nat | 0 <= i < j < |coords| :: (i,j, dist(coords[i], coords[j]));
+        var pairs := MergeSortBy(lte, AllPairs(coords, 0));
+        assert forall p :: p in pairs ==> 0 <= p.0 < p.1 < |coords|;
+        // expect pairs != {};
+        var qu := new QuickUnion(|coords|);
+        assert fresh(qu);
+        var count := 1000-1;
+        while count > 0 && pairs != [] 
+            invariant qu.Valid()
+            invariant fresh(qu)
+            invariant forall p :: p in pairs ==> 0 <= p.0 < p.1 < |coords|
+            invariant qu.n == |coords|
+            modifies qu
+            decreases *
+        {
+            var nearest := pairs[0];
+            // ThereIsAMinimumTuple(pairs);
+            // var nearest :| nearest in pairs && forall p :: p in pairs ==> nearest.2 <= p.2;
+            // print "\nnearest: ", coords[nearest.0], " ", coords[nearest.1], " ", nearest.2;
+            var areConnected := qu.connected(nearest.0, nearest.1);
+            // print "\nareConnected: ", areConnected;
+            if !areConnected {
+                qu.union(nearest.0, nearest.1);
+                if count == 1 {
+                    return coords[nearest.0].0 * coords[nearest.1].0;
+                }
+                count := count - 1;
+            }
+            pairs:= pairs[1..];
+
+        }
     }
 }
